term subst: finish subtyping

Capless/Subst/Basic.lean
@@ -2,11 +2,113 @@ import Capless.Basic
 import Capless.Context
 import Capless.CaptureSet
 import Capless.Typing
+import Capless.Renaming.Term.Typing
+import Capless.Renaming.Type.Typing
+import Capless.Renaming.Capture.Typing
 namespace Capless
 
 structure VarSubst (Γ : Context n m k) (f : FinFun n n') (Δ : Context n' m k) where
   map : ∀ x E, Γ.Bound x E -> Typed Δ (Term.var (f x)) (EType.type (E.rename f))
   tmap : ∀ X b, Γ.TBound X b -> Δ.TBound X (b.rename f)
   cmap : ∀ c b, Γ.CBound c b -> Δ.CBound c (b.rename f)
+
+def VarSubst.ext {Γ : Context n m k}
+  (σ : VarSubst Γ f Δ)
+  (T : CType n m k) :
+  VarSubst (Γ.var T) f.ext (Δ.var (T.rename f)) := by
+  constructor
+  case map =>
+    intros x E hb
+    cases hb
+    case here =>
+      simp [FinFun.ext]
+      apply Typed.var
+      rw [<- CType.weaken_rename]
+      constructor
+    case there_var hb0 =>
+      simp [FinFun.ext]
+      rw [<- CType.weaken_rename]
+      have h0 := σ.map _ _ hb0
+      have h1 := Typed.weaken h0 (T := T.rename f)
+      simp [Term.weaken, Term.rename, FinFun.weaken] at h1
+      simp [EType.weaken, EType.rename, CType.weaken] at *
+      exact h1
+  case tmap =>
+    intros X b hb
+    cases hb
+    case there_var hb0 =>
+      have hb1 := σ.tmap _ _ hb0
+      rw [<- TBinding.weaken_rename]
+      constructor; trivial
+  case cmap =>
+    intros x b hb
+    cases hb
+    case there_var hb0 =>
+      have hb1 := σ.cmap _ _ hb0
+      rw [<- CBinding.weaken_rename]
+      constructor; trivial
+
+def VarSubst.text {Γ : Context n m k}
+  (σ : VarSubst Γ f Δ) :
+  VarSubst (Γ.tvar b) f (Δ.tvar (b.rename f)) := by
+  constructor
+  case map =>
+    intros x T hb
+    cases hb
+    case there_tvar hb0 =>
+      have h0 := σ.map _ _ hb0
+      have h1 := h0.tweaken (b := (b.rename f))
+      rw [CType.tweaken_rename]
+      simp [EType.tweaken, EType.trename,
+            CType.tweaken, Term.tweaken, Term.trename] at *
+      exact h1
+  case tmap =>
+    intros X b hb
+    cases hb
+    case here =>
+      rw [TBinding.tweaken_rename_comm]
+      constructor
+    case there_tvar hb0 =>
+      have hb1 := σ.tmap _ _ hb0
+      rw [TBinding.tweaken_rename_comm]
+      constructor; trivial
+  case cmap =>
+    intros c b hb
+    cases hb
+    case there_tvar hb0 =>
+      have hb1 := σ.cmap _ _ hb0
+      constructor; trivial
+
+def VarSubst.cext {Γ : Context n m k}
+  (σ : VarSubst Γ f Δ) :
+  VarSubst (Γ.cvar b) f (Δ.cvar (b.rename f)) := by
+  constructor
+  case map =>
+    intros x T hb
+    cases hb
+    case there_cvar hb0 =>
+      have h0 := σ.map _ _ hb0
+      have h1 := h0.cweaken (b := (b.rename f))
+      rw [CType.cweaken_rename_comm]
+      simp [EType.cweaken, EType.crename,
+            CType.cweaken, Term.cweaken, Term.crename] at *
+      exact h1
+  case tmap =>
+    intros X b hb
+    cases hb
+    case there_cvar hb0 =>
+      have hb1 := σ.tmap _ _ hb0
+      rw [TBinding.cweaken_rename_comm]
+      constructor; trivial
+  case cmap =>
+    intros c b hb
+    cases hb
+    case here =>
+      rw [CBinding.cweaken_rename_comm]
+      constructor
+    case there_cvar hb0 =>
+      have hb1 := σ.cmap _ _ hb0
+      rw [CBinding.cweaken_rename_comm]
+      constructor; trivial
 
 end Capless
