Capless/Renaming/Basic.lean
@@ -289,4 +289,16 @@ theorem Finset.DropBinder.rename
     apply drop
     apply DropBinderFree.rename; assumption
 
+def VarMap.weaken {Γ : Context n m k} :
+  VarMap Γ FinFun.weaken (Γ.var T) := by
+  constructor <;> (intros; constructor; trivial)
+
+def CVarMap.weaken {Γ : Context n m k} :
+  CVarMap Γ FinFun.weaken (Γ.cvar b) := by
+  constructor <;> (intros; constructor; trivial)
+
+def TVarMap.weaken {Γ : Context n m k} :
+  TVarMap Γ FinFun.weaken (Γ.tvar b) := by
+  constructor <;> (intros; constructor; trivial)
+
 end Capless
