Capless/Renaming/Capture/Typing.lean
@@ -220,4 +220,11 @@ theorem Typed.crename
     rw [<- EType.cweaken_crename] at ih
     exact ih
 
+def Typed.cweaken
+  (h : Typed Γ t E) :
+  Typed (Γ.cvar b) t.cweaken E.cweaken := by
+  simp [Term.cweaken, EType.cweaken]
+  apply h.crename
+  apply CVarMap.weaken
+
 end Capless
