Capless/Subst/Term/Typing.lean
@@ -1,0 +1,10 @@
+import Capless.Typing
+import Capless.Subst.Basic
+namespace Capless
+
+theorem Typed.subst
+  (h : Typed Γ t E)
+  (σ : VarSubst Γ f Δ) :
+  Typed Δ (t.rename f) (E.rename f) := sorry
+
+end Capless
